I understand that the recursive approach can be a bit tricky to grasp at first. Let's try to break it down further with a more detailed example.

Consider the following linked list:

1 -> 2 -> 3 -> 4 -> NULL
Recursive Call 1:

Base Case Check: The function checks if the head is NULL or if the next node is NULL. In this case, it's not, so we move to the recursive case.
Recursive Call: The function calls itself with head->next as the new head. This means it's now trying to reverse the sublist 2 -> 3 -> 4.
Rewiring: After the recursive call returns, the function rewires the links:
It sets the next pointer of node 2 to point to node 1.
It sets the next pointer of node 1 to NULL.
After the first recursive call, the list looks like this:

1 <- 2 -> 3 -> 4 -> NULL
Recursive Call 2:

Base Case Check: The function checks if the head (which is now 2) is NULL or if the next node is NULL. It's not, so we move to the recursive case.
Recursive Call: The function calls itself with head->next (which is 3) as the new head. This means it's now trying to reverse the sublist 3 -> 4.
Rewiring: After the recursive call returns, the function rewires the links:
It sets the next pointer of node 3 to point to node 2.
It sets the next pointer of node 2 to NULL.
After the second recursive call, the list looks like this:

1 <- 2 <- 3 -> 4 -> NULL
Recursive Call 3:

Base Case Check: The function checks if the head (which is now 3) is NULL or if the next node is NULL. It's not, so we move to the recursive case.
Recursive Call: The function calls itself with head->next (which is 4) as the new head.
Rewiring: After the recursive call returns, the function rewires the links:
It sets the next pointer of node 4 to point to node 3.
It sets the next pointer of node 3 to NULL.
After the third recursive call, the list looks like this:

1 <- 2 <- 3 <- 4 -> NULL
Now, the recursion unwinds, and we have the final reversed linked list:

4 -> 3 -> 2 -> 1 -> NULL
Key Point:

The magic of recursion lies in breaking down a complex problem into smaller, simpler subproblems. In this case, the problem of reversing a linked list is broken down into reversing smaller sublists. The base case ensures that the recursion eventually stops when the simplest case (a list with one or no nodes) is reached.

I hope this explanation is clearer. If you have any more questions, feel free to ask!
